src/ch7_cont.lean
@@ -1,0 +1,616 @@
+import ch6_cont
+universe u
+namespace Set
+
+local attribute [irreducible] mem
+
+-- chapter 7 exercise 20
+lemma finite_of_well_orderings {A R : Set} (Rwell : A.well_order R) (Rwell' : A.well_order R.inv) : A.is_finite :=
+begin
+  have eg : ∀ {X : Set}, X ≠ ∅ → X ⊆ A → ∃ m : Set, m ∈ X ∧ ∀ {x : Set}, x ∈ X → R.lin_le x m,
+    intros X XE XA, obtain ⟨m, mX, ge⟩ := Rwell'.well XE XA,
+    rw [is_least] at ge, push_neg at ge, refine ⟨_, mX, λ x, assume xX, _⟩,
+    rw le_iff_not_lt Rwell.lin (XA xX) (XA mX),
+    specialize ge _ xX, rw pair_mem_inv at ge, exact ge,
+  let closed := λ X : Set, ∀ {y : Set}, y ∈ X → ∀ {x : Set}, x.pair y ∈ R → x ∈ X,
+  have un : ∀ {X : Set}, X ≠ ∅ → X ⊆ A → closed X → ∃ m : Set, m ∈ X ∧ X = (R.seg m) ∪ {m},
+    intros X XE XA cl, obtain ⟨m, mX, ge⟩ := eg XE XA, refine ⟨m, mX, _⟩,
+    apply ext, intro x, rw [mem_union, mem_singleton, mem_seg, ←lin_le], split,
+      exact ge, rintro (xm|xm),
+        exact cl mX xm,
+      subst xm, exact mX,
+  have segcl : ∀ {t : Set}, t ∈ A → closed (R.seg t), intros t tA y yt x xy,
+    rw mem_seg at *, exact Rwell.lin.trans xy yt,
+  have segsub : ∀ {t : Set}, t ∈ A → R.seg t ⊆ A, intros t tA x xt,
+    rw mem_seg at xt, replace xt := Rwell.lin.rel xt, rw pair_mem_prod at xt,
+    exact xt.left,
+  have Acl : closed A, intros y yA x xy, replace xy := Rwell.lin.rel xy,
+    rw pair_mem_prod at xy, exact xy.left,
+  let B := {x ∈ A | (R.seg x).is_finite},
+  have BA : B = A, apply transfinite_ind Rwell sep_subset,
+    intros x xA ind, rw mem_sep,
+    by_cases se : R.seg x = ∅,
+      rw [se, ←card_finite_iff_finite, card_nat zero_nat, finite_cardinal_iff_nat],
+      exact ⟨xA, zero_nat⟩,
+    obtain ⟨m, mx, eq⟩ := un se (segsub xA) (@segcl _ xA), rw eq,
+    specialize ind mx, rw mem_sep at ind,
+    exact ⟨xA, union_finite_of_finite ind.right singleton_finite⟩,
+  by_cases Ae : A = ∅,
+    subst Ae, rw [←card_finite_iff_finite, card_nat zero_nat, finite_cardinal_iff_nat],
+    exact zero_nat,
+  obtain ⟨m, mx, eq⟩ := un Ae subset_self @Acl, rw eq, rw [←BA, mem_sep] at mx,
+  exact union_finite_of_finite mx.right singleton_finite,
+end
+
+-- end of chapter 7 starting from page 199
+
+lemma card_is_ord {κ : Set} (κcard : κ.is_cardinal) : κ.is_ordinal :=
+begin
+  rcases κcard with ⟨K, Kcard⟩, rw ←Kcard, exact card_is_ordinal,
+end
+
+lemma card_is_ord' {A : Set} : A.card.is_ordinal :=
+card_is_ord ⟨_, rfl⟩
+
+lemma card_lt_of_mem {κ : Set} (κcard : κ.is_cardinal) {μ : Set} (μcard : μ.is_cardinal) (κμ : κ ∈ μ) : κ.card_lt μ :=
+begin
+  have κord := card_is_ord κcard,
+  have μord := card_is_ord μcard,
+  rw ord_mem_iff_ssub κord μord at κμ,
+  rw card_lt, refine ⟨_, κμ.right⟩,
+  rw [←card_of_cardinal_eq_self κcard, ←card_of_cardinal_eq_self μcard],
+  exact card_le_of_subset κμ.left,
+end
+
+lemma not_card_lt_of_not_mem {κ : Set} (κcard : κ.is_cardinal) {μ : Set} (μcard : μ.is_cardinal) (κμ : κ ∉ μ) : ¬ κ.card_lt μ :=
+begin
+  have κord := card_is_ord κcard,
+  have μord := card_is_ord μcard,
+  rw ←ord_not_le_iff_lt μord κord at κμ, push_neg at κμ,
+  have μκ : μ.card_le κ, cases κμ,
+      exact (card_lt_of_mem μcard κcard κμ).left,
+    subst κμ, exact card_le_refl,
+  intro lt,
+  exact lt.right (card_eq_of_le_of_le κcard μcard lt.left μκ),
+end
+
+lemma card_lt_iff_mem {κ : Set} (κcard : κ.is_cardinal) {μ : Set} (μcard : μ.is_cardinal) : κ.card_lt μ ↔ κ ∈ μ :=
+⟨λ κμ, classical.by_contradiction (λ nκμ, (not_card_lt_of_not_mem κcard μcard nκμ) κμ), card_lt_of_mem κcard μcard⟩
+
+lemma card_le_iff_le {κ : Set} (κcard : κ.is_cardinal) {μ : Set} (μcard : μ.is_cardinal) : κ.card_le μ ↔ κ ≤ μ :=
+by rw [card_le_iff, le_iff, card_lt_iff_mem κcard μcard]
+
+lemma ord_dom_of_le {α : Set} (αord : α.is_ordinal) {β : Set} (βord : β.is_ordinal)
+  (αβ : α ≤ β) : α ≼ β :=
+begin
+  rw ord_le_iff_sub αord βord at αβ, rw dominated_iff,
+  exact ⟨_, αβ, equin_refl⟩,
+end
+
+lemma ord_lt_of_card_lt {α : Set} (αord : α.is_ordinal) {β : Set} (βord : β.is_ordinal)
+  (lt : α.card.card_lt β.card) : α ∈ β :=
+begin
+  rw card_lt_iff at lt, rw ←ord_not_le_iff_lt βord αord, intro le, apply lt.right,
+  exact equin_of_dom_of_dom lt.left (ord_dom_of_le βord αord le),
+end
+
+-- problem 24 lemma
+lemma ord_mem_card_powerset {α : Set} (αord : α.is_ordinal) : α ∈ α.powerset.card :=
+begin
+  apply ord_lt_of_card_lt αord card_is_ord', rw [card_of_cardinal_eq_self ⟨_, rfl⟩, card_power],
+  exact card_lt_exp ⟨_, rfl⟩,
+end
+
+-- problem 24
+lemma exists_larger_card {α : Set} (αord : α.is_ordinal) : ∃ κ : Set, κ.is_cardinal ∧ α ∈ κ :=
+⟨_, ⟨_, rfl⟩, ord_mem_card_powerset αord⟩
+
+-- problem 25
+lemma trans_ind_schema {φ : Set → Prop} (ind : ∀ {α : Set}, α.is_ordinal → (∀ {x : Set}, x ∈ α → φ x) → φ α)
+  (α : Set) (αord : α.is_ordinal) : φ α :=
+begin
+  let X := {x ∈ α.succ | φ x},
+  have Xα : X = α.succ,
+    apply transfinite_ind (ordinal_well_ordered (succ_ord_of_ord αord)) sep_subset,
+    intros t tα hi, rw mem_sep, refine ⟨tα, ind (ord_of_mem_ord (succ_ord_of_ord αord) tα) _⟩,
+    intros x xt,
+    suffices xX : x ∈ X, rw mem_sep at xX, exact xX.right,
+    apply hi, rw [mem_seg, eps_order, pair_mem_pair_sep' (ord_mem_trans (succ_ord_of_ord αord) xt tα) tα],
+    exact xt,
+  suffices h : α ∈ X, rw mem_sep at h, exact h.right,
+  rw Xα, exact self_mem_succ,
+end
+
+def init_ord (α : Set) : Prop := α.is_ordinal ∧ ¬ ∃ β : Set, β ∈ α ∧ α ≈ β
+
+theorem init_iff_card {α : Set} : α.init_ord ↔ α.is_cardinal :=
+begin
+  split,
+    intro init, use α, symmetry, apply eq_card init.left equin_refl,
+    intros β βord αβ, apply classical.by_contradiction, intro le,
+    rw ord_not_le_iff_lt init.left βord at le, exact init.right ⟨_, le, αβ⟩,
+  intro αcard,
+  have eq := card_of_cardinal_eq_self αcard, rw ←eq, refine ⟨card_is_ordinal, _⟩,
+  rintro ⟨β, βA, Aβ⟩,
+  have βord := ord_of_mem_ord card_is_ordinal βA,
+  rw ←ord_not_le_iff_lt card_is_ordinal βord at βA,
+  rw eq at Aβ, apply βA, exact card_least βord Aβ,
+
+end
+
+lemma omega_is_card : is_cardinal ω :=
+begin
+  rw ←init_iff_card, split,
+    exact omega_is_ord,
+  rintro ⟨n, nω, ωn⟩, exact nat_infinite ⟨_, nω, ωn⟩,
+end
+
+lemma exists_powersets (X : Set) : ∃ B : Set, ∀ (y : Set), y ∈ B ↔ ∃ x : Set, x ∈ X ∧ y = x.powerset :=
+replacement'' powerset
+noncomputable def powersets (X : Set.{u}) : Set.{u} := classical.some X.exists_powersets
+lemma mem_powersets {X y : Set} : y ∈ X.powersets ↔ ∃ x : Set, x ∈ X ∧ y = x.powerset :=
+classical.some_spec X.exists_powersets y
+
+lemma L7Q {δ : Set} (δord : δ.is_ordinal) :
+  ∃ F : Set, F.is_function ∧ F.dom = δ ∧ ∀ ⦃α : Set⦄, α ∈ δ → F.fun_value α = ((F.img α).powersets).Union :=
+begin
+  obtain ⟨F, Ffun, Fdom, Fspec⟩ := exists_of_exists_unique (@transfinite_rec' δ δ.eps_order (ordinal_well_ordered δord) (fun x, x.ran.powersets.Union)),
+  refine ⟨_, Ffun, Fdom, λ α αδ, _⟩, specialize Fspec αδ, rw Fspec,
+  dsimp, rw [restrict_ran, seg_eq_of_trans (ordinal_trans δord) αδ],
+end
+
+local attribute [instance] classical.prop_decidable
+
+noncomputable def L7Q_fun (δ : Set) : Set := if δord : δ.is_ordinal then classical.some (L7Q δord) else ∅
+lemma L7Q_fun_spec {δ : Set} (δord : δ.is_ordinal) :
+  δ.L7Q_fun.is_function ∧ δ.L7Q_fun.dom = δ ∧ ∀ ⦃α : Set⦄, α ∈ δ → δ.L7Q_fun.fun_value α = ((δ.L7Q_fun.img α).powersets).Union :=
+begin
+  simp [L7Q_fun, dif_pos δord], exact classical.some_spec (L7Q δord),
+end
+
+lemma L7R : ∀ {δ : Set}, δ.is_ordinal → ∀ {ε : Set}, ε.is_ordinal →
+  ∀ {α : Set}, α ∈ δ ∩ ε → δ.L7Q_fun.fun_value α = ε.L7Q_fun.fun_value α :=
+begin
+  have h₁ : ∀ {δ : Set}, δ.is_ordinal → ∀ {α : Set}, α ∈ δ → ∀ {z : Set}, z ∈ (δ.L7Q_fun.img α).powersets ↔ ∃ β : Set, β ∈ α ∧ z = (δ.L7Q_fun.fun_value β).powerset,
+    intros δ δord α αδ z, rw mem_powersets,
+    have αord : α.is_ordinal := ord_of_mem_ord δord αδ,
+    rw ord_mem_iff_ssub αord δord at αδ,
+    obtain ⟨δfun, δdom, -⟩ := L7Q_fun_spec δord, rw ←δdom at αδ, simp only [mem_img' δfun αδ.left], split,
+      rintro ⟨y, ⟨β, βα, yfβ⟩, zy⟩, subst yfβ, exact ⟨_, βα, zy⟩,
+    rintro ⟨β, βα, zf⟩, exact ⟨_, ⟨_, βα, rfl⟩, zf⟩,
+  have h₂ : ∀ {δ : Set}, δ.is_ordinal → ∀ {ε : Set}, ε.is_ordinal → δ ⊆ ε → {α ∈ δ | δ.L7Q_fun.fun_value α = ε.L7Q_fun.fun_value α} = δ,
+    intros δ δord ε εord δε, apply transfinite_ind (ordinal_well_ordered δord) sep_subset,
+    obtain ⟨-, -, δspec⟩ := L7Q_fun_spec δord, obtain ⟨-, -, εspec⟩ := L7Q_fun_spec εord,
+    intros α αδ ind, rw [mem_sep, δspec αδ, εspec (δε αδ)], refine ⟨αδ, _⟩,
+    congr' 1, apply ext, simp only [h₁ δord αδ, h₁ εord (δε αδ)], intro z, apply exists_congr,
+    intro β, rw and.congr_right_iff, intro βα,
+    suffices hβ : β ∈ δ.eps_order.seg α, specialize ind hβ, rw mem_sep at ind, rw ind.right,
+    rw [mem_seg, eps_order, pair_mem_pair_sep' (ord_mem_trans δord βα αδ) αδ], exact βα,
+  intros δ δord ε εord α hα, cases ord_conn' δord εord,
+    rw ord_le_iff_sub δord εord at h, rw inter_eq_of_sub h at hα,
+    specialize h₂ δord εord h, rw [←h₂, mem_sep] at hα, exact hα.right,
+  rw ord_le_iff_sub εord δord at h, rw [inter_comm, inter_eq_of_sub h] at hα,
+  specialize h₂ εord δord h, rw [←h₂, mem_sep] at hα, exact hα.right.symm,
+end
+
+noncomputable def Veb (α : Set) : Set := α.succ.L7Q_fun.fun_value α
+noncomputable def Veb_img (α : Set) : Set :=
+classical.some (@replacement'' Veb α)
+lemma mem_Veb_img {α V : Set} : V ∈ α.Veb_img ↔ ∃ β : Set, β ∈ α ∧ V = β.Veb :=
+classical.some_spec (@replacement'' Veb α)
+
+-- Theorem 7S
+theorem Veb_eq {α : Set} (αord : α.is_ordinal) : α.Veb = α.Veb_img.powersets.Union :=
+begin
+  obtain ⟨f, dom, spec⟩ := L7Q_fun_spec (succ_ord_of_ord αord),
+  rw [Veb, spec self_mem_succ], congr, apply ext, intro V,
+  have subdom : α ⊆ α.succ.L7Q_fun.dom, rw dom, exact self_sub_succ,
+  simp only [mem_img' f subdom, mem_Veb_img, Veb], apply exists_congr,
+  intro β, rw and.congr_right_iff, intro βα, apply eq.congr_right,
+  apply L7R (succ_ord_of_ord αord) (succ_ord_of_ord (ord_of_mem_ord αord βα)),
+  rw mem_inter, refine ⟨_, self_mem_succ⟩, rw [succ, mem_union], right, exact βα,
+end
+
+lemma mem_Veb {α : Set} (αord : α.is_ordinal) {X : Set} : X ∈ α.Veb ↔ ∃ β : Set, β ∈ α ∧ X ⊆ β.Veb :=
+begin
+  simp only [Veb_eq αord, mem_Union, exists_prop, mem_powersets, mem_Veb_img], split,
+    rintro ⟨Y, ⟨V, ⟨β, βα, Vβ⟩, YV⟩, XY⟩, subst Vβ, subst YV, rw mem_powerset at XY, exact ⟨_, βα, XY⟩,
+  rintro ⟨β, βα, Xβ⟩, refine ⟨_, ⟨_, ⟨_, βα, rfl⟩, rfl⟩, _⟩, rw mem_powerset, exact Xβ,
+end
+
+-- Theorem 7T
+theorem Veb_transitive : ∀ {α : Set}, α.is_ordinal → α.Veb.transitive_set :=
+begin
+  refine trans_ind_schema _, intros α αord hi, rw transitive_set_iff', intros X XV,
+  simp only [Veb_eq αord, mem_Union, exists_prop, mem_powersets, mem_Veb_img] at XV,
+  rcases XV with ⟨S, ⟨V, ⟨β, βα, Vβ⟩, SV⟩, XS⟩, subst SV, subst Vβ,
+  have h := powerset_transitive (hi βα), rw transitive_set_iff' at h,
+  specialize h XS, apply subset_trans h, intros Z Zβ,
+  simp only [Veb_eq αord, mem_Union, exists_prop, mem_powersets, mem_Veb_img],
+  exact ⟨_, ⟨_, ⟨_, βα, rfl⟩, rfl⟩, Zβ⟩,
+end
+
+structure limit_ord (α : Set) : Prop :=
+(ord : α.is_ordinal)
+(ne : α ≠ ∅)
+(ns : ¬ ∃ β : Set, α = β.succ)
+
+lemma succ_mem_limit {γ : Set} (γord : γ.limit_ord) {β : Set} (βγ : β ∈ γ) : β.succ ∈ γ :=
+begin
+  cases succ_least_upper_bound γord.ord βγ,
+    exact h,
+  exfalso, exact γord.ns ⟨_, h.symm⟩,
+end
+
+lemma limit_ord_inf {γ : Set} (γord : γ.limit_ord) : ¬ γ.is_finite :=
+begin
+  apply inf_of_sup_inf nat_infinite, rw subset_def,
+  apply induction,
+    rw ←ord_not_le_iff_lt γord.ord (nat_is_ord zero_nat), rintro (h|h),
+      exact mem_empty _ h,
+    exact γord.ne h,
+  intros n nω nγ, exact succ_mem_limit γord nγ,
+end
+
+-- Theorem 7U part a
+theorem Veb_sub_of_mem {β α : Set} (αord : α.is_ordinal) (βα : β ∈ α) : β.Veb ⊆ α.Veb :=
+begin
+  intros X Xβ, rw mem_Veb αord,
+  have βord := ord_of_mem_ord αord βα,
+  have trans := Veb_transitive βord, rw transitive_set_iff' at trans,
+  exact ⟨_, βα, trans Xβ⟩,
+end
+
+-- Theorem 7U part b
+theorem Veb_null_eq_null : Veb ∅ = ∅ :=
+begin
+  rw eq_empty, intros z zV, rw mem_Veb zero_is_ord at zV,
+  rcases zV with ⟨β, βn, -⟩, exact mem_empty _ βn,
+end
+
+-- Theorem 7U part c
+theorem Veb_succ_eq_powerset {α : Set} (αord : α.is_ordinal) : α.succ.Veb = α.Veb.powerset :=
+begin
+  apply ext, simp only [mem_Veb (succ_ord_of_ord αord), mem_powerset], intro X, split,
+    rintro ⟨β, βα, Xβ⟩, rw [succ, mem_union, mem_singleton] at βα, cases βα,
+      subst βα, exact Xβ,
+    exact subset_trans Xβ (Veb_sub_of_mem αord βα),
+  intro Xα, exact ⟨_, self_mem_succ, Xα⟩,
+end
+
+lemma mem_Union_Veb_img {α X : Set} : X ∈ α.Veb_img.Union ↔ ∃ β : Set, β ∈ α ∧ X ∈ β.Veb :=
+begin
+  simp only [mem_Union, exists_prop, mem_Veb_img], split,
+    rintro ⟨V, ⟨β, βα, Vβ⟩, XV⟩, subst Vβ, exact ⟨_, βα, XV⟩,
+  rintro ⟨β, βα, Xβ⟩, exact ⟨_, ⟨_, βα, rfl⟩, Xβ⟩,
+end
+
+-- Theorem 7U part d
+theorem Veb_limit_ord_eq {γ : Set} (γord : γ.limit_ord) : γ.Veb = γ.Veb_img.Union :=
+begin
+  apply ext, simp only [mem_Veb γord.ord, mem_Union_Veb_img], intro X, split,
+    rintro ⟨β, βγ, Xβ⟩, refine ⟨_, succ_mem_limit γord βγ, _⟩,
+    rw [Veb_succ_eq_powerset (ord_of_mem_ord γord.ord βγ), mem_powerset], exact Xβ,
+  rintro ⟨β, βγ, Xβ⟩,
+  have trans := Veb_transitive (ord_of_mem_ord γord.ord βγ),
+  rw transitive_set_iff' at trans, exact ⟨_, βγ, trans Xβ⟩,
+end
+
+lemma exists_least_ord_of_exists {p : Set → Prop} (h : ∃ α : Set, α.is_ordinal ∧ p α) :
+  ∃ α : Set, α.is_ordinal ∧ p α ∧ ∀ {β : Set}, β.is_ordinal → p β → α ≤ β :=
+begin
+  rcases h with ⟨α, αord, pα⟩,
+  have αord' := succ_ord_of_ord αord,
+  let X := {β ∈ α.succ | p β},
+  have XE : X ≠ ∅, apply ne_empty_of_inhabited, use α, rw mem_sep, exact ⟨self_mem_succ, pα⟩,
+  obtain ⟨γ, γX, h⟩ := (ordinal_well_ordered αord').well XE sep_subset,
+  rw mem_sep at γX, refine ⟨_, ord_of_mem_ord αord' γX.left, γX.right, λ β, assume βord pβ, _⟩,
+  apply classical.by_contradiction, intro γβ, apply h, use β,
+  rw ord_not_le_iff_lt (ord_of_mem_ord αord' γX.left) βord at γβ,
+  have βα := ord_mem_trans αord' γβ γX.left,
+  rw [mem_sep, eps_order, pair_mem_pair_sep' βα γX.left],
+  exact ⟨⟨βα, pβ⟩, γβ⟩,
+end
+
+def grounded (A : Set) : Prop := ∃ α : Set, α.is_ordinal ∧ A ⊆ α.Veb
+
+noncomputable def rank (A : Set) : Set := if h : A.grounded then classical.some (exists_least_ord_of_exists h) else ∅
+lemma rank_ord_of_grounded {A : Set} (Agr : A.grounded) : A.rank.is_ordinal :=
+begin
+  simp only [rank, dif_pos Agr],
+  obtain ⟨h, -, -⟩ := classical.some_spec (exists_least_ord_of_exists Agr),
+  exact h,
+end
+lemma rank_sub_of_grounded {A : Set} (Agr : A.grounded) : A ⊆ A.rank.Veb :=
+begin
+  simp only [rank, dif_pos Agr],
+  obtain ⟨-, h, -⟩ := classical.some_spec (exists_least_ord_of_exists Agr),
+  exact h,
+end
+lemma rank_least_of_grounded {A : Set} (Agr : A.grounded) : ∀ {β : Set}, β.is_ordinal → A ⊆ β.Veb → A.rank ≤ β :=
+begin
+  simp only [rank, dif_pos Agr],
+  obtain ⟨-, -, h⟩ := classical.some_spec (exists_least_ord_of_exists Agr),
+  exact @h,
+end
+
+lemma ord_not_sub_Veb {α : Set} (αord : α.is_ordinal) : ∀ {β : Set}, β ∈ α → ¬ (α ⊆ β.Veb) :=
+begin
+  revert α, refine trans_ind_schema _, intros α αord ind β βα αβ,
+  suffices ββ : β ∉ β.Veb,
+    exact ββ (αβ βα),
+  rw mem_Veb (ord_of_mem_ord αord βα), rintro ⟨δ, δβ, βδ⟩,
+  exact ind βα δβ βδ,
+end
+
+lemma ord_sub_Veb_self {α : Set} (αord : α.is_ordinal) : α ⊆ α.Veb :=
+begin
+  revert α, refine trans_ind_schema _, intros α αord ind β βα,
+  specialize ind βα, rw mem_Veb αord, exact ⟨_, βα, ind⟩,
+end
+
+-- exercise 26
+theorem ord_grounded {α : Set} (αord : α.is_ordinal) : α.grounded := ⟨_, αord, ord_sub_Veb_self αord⟩
+theorem rank_ord_eq_self {α : Set} (αord : α.is_ordinal) : α.rank = α :=
+begin
+  have h := rank_least_of_grounded (ord_grounded αord) αord (ord_sub_Veb_self αord),
+  cases h,
+    exfalso, exact ord_not_sub_Veb αord h (rank_sub_of_grounded (ord_grounded αord)),
+  exact h,
+end
+
+-- Theorem 7V part a part 1
+theorem grounded_of_mem_grounded {A : Set} (Agr : A.grounded) {a : Set} (aA : a ∈ A) : a.grounded :=
+begin
+  obtain ⟨α, αord, Aα⟩ := Agr,
+  have trans := Veb_transitive αord, rw transitive_set_iff' at trans,
+  exact ⟨_, αord, trans (Aα aA)⟩,
+end
+
+-- Theorem 7V part a part 2
+theorem rank_mem_of_mem_grounded {A : Set} (Agr : A.grounded) {a : Set} (aA : a ∈ A) : a.rank ∈ A.rank :=
+begin
+  have h : a ∈ A.rank.Veb := (rank_sub_of_grounded Agr) aA,
+  have Aord : A.rank.is_ordinal := rank_ord_of_grounded Agr,
+  rw mem_Veb Aord at h, rcases h with ⟨β, βA, aβ⟩,
+  apply @ord_lt_of_le_of_lt _ β _ Aord,
+    exact (rank_least_of_grounded (grounded_of_mem_grounded Agr aA) (ord_of_mem_ord Aord βA) aβ),
+  exact βA,
+end
+
+lemma T7V_ord {A : Set} (hA : ∀ {a : Set}, a ∈ A → a.grounded) : (A.repl_img (succ ∘ rank)).Union.is_ordinal :=
+begin
+  apply Union_ords_is_ord, intros β βA,
+  rw mem_repl_img at βA, rcases βA with ⟨a, aA, βa⟩, subst βa,
+  apply succ_ord_of_ord (rank_ord_of_grounded (hA aA)),
+end
+
+lemma T7V_sub {A : Set} (hA : ∀ {a : Set}, a ∈ A → a.grounded) : A ⊆ (A.repl_img (succ ∘ rank)).Union.Veb :=
+begin
+  intros a aA,
+  have aa : a ∈ a.rank.succ.Veb,
+    rw [Veb_succ_eq_powerset (rank_ord_of_grounded (hA aA)), mem_powerset],
+    exact rank_sub_of_grounded (hA aA),
+  have aα : a.rank.succ ≤ (A.repl_img (succ ∘ rank)).Union,
+    rw ord_le_iff_sub (succ_ord_of_ord (rank_ord_of_grounded (hA aA))) (T7V_ord @hA),
+    apply subset_Union, rw mem_repl_img, exact ⟨_, aA, rfl⟩,
+  cases aα,
+    exact Veb_sub_of_mem (T7V_ord @hA) aα aa,
+  rw ←aα, exact aa,
+end
+
+-- Theorem 7V part b part 1
+theorem grounded_of_all_mem_grounded {A : Set} (hA : ∀ {a : Set}, a ∈ A → a.grounded) : A.grounded :=
+⟨_, T7V_ord @hA, T7V_sub @hA⟩
+
+-- Theorem 7V part b part 2
+theorem rank_eq_of_all_mem_grounded {A : Set} (hA : ∀ {a : Set}, a ∈ A → a.grounded) : A.rank = (A.repl_img (succ ∘ rank)).Union :=
+begin
+  let α := (A.repl_img (succ ∘ rank)).Union,
+  have Agr := grounded_of_all_mem_grounded @hA,
+  rw ord_eq_iff_le_and_le (rank_ord_of_grounded Agr) (T7V_ord @hA), split,
+    exact rank_least_of_grounded Agr (T7V_ord @hA) (T7V_sub @hA),
+  have h₁ : ∀ {a : Set}, a ∈ A → a.rank.succ ≤ A.rank,
+    intros a aA, exact succ_least_upper_bound (rank_ord_of_grounded Agr) (rank_mem_of_mem_grounded Agr aA),
+  have h₂ : ∀ {β : Set}, β.is_ordinal →  (∀ {a : Set}, a ∈ A → a.rank.succ ≤ β) → α ≤ β,
+    intros β βord hβ, rw ord_le_iff_sub (T7V_ord @hA) βord,
+    intro δ, simp only [mem_Union, exists_prop, mem_repl_img],
+    rintro ⟨Z, ⟨a, aA, Za⟩, δZ⟩, subst Za,
+    specialize hβ aA, rw ord_le_iff_sub (succ_ord_of_ord (rank_ord_of_grounded (hA aA))) βord at hβ,
+    exact hβ δZ,
+  exact h₂ (rank_ord_of_grounded Agr) @h₁,
+end
+
+noncomputable def cl_fun (C : Set) : Set :=
+trans_rec ω nat_order (λ f, C ∪ f.ran.Union.Union)
+lemma cl_fun_fun {C : Set} : C.cl_fun.is_function := trans_rec_fun nat_well_order'
+lemma cl_fun_dom {C : Set} : C.cl_fun.dom = ω := trans_rec_dom nat_well_order'
+
+-- problem 7(b)
+lemma cl_fun_lemma {C n : Set} (nω : n ∈ ω) {a : Set} (an : a ∈ C.cl_fun.fun_value n) : a ⊆ C.cl_fun.fun_value n.succ :=
+begin
+  have nω' := nat_induct.succ_closed nω,
+  rw [cl_fun, trans_rec_spec nat_well_order' nω', nat_order_seg nω', restrict_ran],
+  have h : n.succ ⊆ (trans_rec ω nat_order (λ f, C ∪ f.ran.Union.Union)).dom,
+    rw trans_rec_dom nat_well_order', exact subset_nat_of_mem_nat nω',
+  apply subset_union_of_subset_right, apply subset_Union,
+  simp only [mem_Union, exists_prop, mem_img' (trans_rec_fun nat_well_order') h],
+  rw cl_fun at an, exact ⟨_, ⟨_, self_mem_succ, rfl⟩, an⟩,
+end
+
+-- problem 7(c)
+noncomputable def trans_cl (C : Set) : Set := C.cl_fun.ran.Union
+lemma trans_cl_sub {C : Set} : C ⊆ C.trans_cl :=
+begin
+  apply subset_Union, simp only [cl_fun, mem_ran_iff (trans_rec_fun nat_well_order'), trans_rec_dom nat_well_order'], use ∅,
+  simp only [trans_rec_spec nat_well_order' zero_nat, nat_order_seg zero_nat, restrict_empty, ran_empty_eq_empty, union_empty_eq_empty, union_empty],
+  exact ⟨zero_nat, rfl⟩,
+end
+lemma trans_cl_trans {C : Set} : C.trans_cl.transitive_set :=
+begin
+  rw transitive_set_iff', intros a aC,
+  simp only [trans_cl, mem_Union, exists_prop, mem_ran_iff cl_fun_fun, cl_fun_dom] at aC,
+  rcases aC with ⟨y, ⟨n, nω, yn⟩, ay⟩, subst yn,
+  replace ay := cl_fun_lemma nω ay,
+  apply subset_trans ay, simp only [subset_def, trans_cl, mem_Union, exists_prop, mem_ran_iff cl_fun_fun, cl_fun_dom],
+  intros y yn, exact ⟨_, ⟨_, nat_induct.succ_closed nω, rfl⟩, yn⟩,
+end
+
+def reg_axiom : Prop := ∀ {A : Set}, A ≠ ∅ → ∃ m : Set, m ∈ A ∧ m ∩ A = ∅
+
+-- Theorem 7W
+theorem all_grounded_equiv_reg : (∀ {A : Set.{u}}, A.grounded) ↔ reg_axiom.{u} :=
+begin
+  split,
+    intros gr A Ane,
+    let B := A.repl_img rank,
+    have Bord : ∀ x : Set, x ∈ B → x.is_ordinal, simp only [mem_repl_img],
+      rintros μ ⟨x, xA, μx⟩, subst μx, exact rank_ord_of_grounded gr,
+    have Bne : B ≠ ∅, apply ne_empty_of_inhabited,
+      replace Ane := inhabited_of_ne_empty Ane, rcases Ane with ⟨x, xA⟩,
+      use x.rank, rw mem_repl_img, exact ⟨_, xA, rfl⟩,
+    obtain ⟨μ, μB, le⟩ := exists_least_ord_of_nonempty Bord Bne,
+    rw mem_repl_img at μB, rcases μB with ⟨m, mA, μm⟩, subst μm,
+    refine ⟨_, mA, _⟩, rw eq_empty, intros x xmA, rw mem_inter at xmA,
+    apply le, use x.rank, simp only [mem_repl_img, eps_order, pair_mem_pair_sep],
+    exact ⟨⟨_, xmA.right, rfl⟩, ⟨_, xmA.right, rfl⟩, ⟨_, mA, rfl⟩, rank_mem_of_mem_grounded gr xmA.left⟩,
+  intros reg, apply @classical.by_contradiction (∀ {A : Set}, A.grounded), intro h,
+  push_neg at h, rcases h with ⟨c, cng⟩,
+  let B := trans_cl {c},
+  let A : Set := {x ∈ B | ¬ x.grounded},
+  have Ane : A ≠ ∅, apply ne_empty_of_inhabited, use c, rw mem_sep, refine ⟨trans_cl_sub _, cng⟩,
+    rw mem_singleton,
+  obtain ⟨m, mA, miA⟩ := reg Ane,
+  rw mem_sep at mA, apply mA.right, apply grounded_of_all_mem_grounded,
+  intros x xm,
+  have trans : B.transitive_set := trans_cl_trans, rw transitive_set_iff at trans,
+  have xB : x ∈ B := trans mA.left xm,
+  have xA : x ∉ A, intro xA, apply mem_empty x, rw [←miA, mem_inter], exact ⟨xm, xA⟩,
+  rw mem_sep at xA, push_neg at xA, exact xA xB,
+end
+
+-- A proof of the regularity axiom
+theorem regularity' : reg_axiom :=
+begin
+  intros A Ane,
+  have h := regularity _ Ane,
+  simp only [exists_prop] at h, simp only [inter_comm], exact h,
+end
+
+theorem all_grounded : ∀ {x : Set}, x.grounded :=
+begin
+  rw all_grounded_equiv_reg, exact @regularity',
+end
+
+-- Theorem 7X(a)
+theorem not_mem_self {A : Set} : A ∉ A :=
+begin
+  intro AA,
+  obtain ⟨m, mA, miA⟩ := regularity' (@singleton_ne_empty A),
+  rw mem_singleton at mA, subst mA,
+  apply mem_empty m, rw [←miA, mem_inter, mem_singleton], exact ⟨AA, rfl⟩,
+end
+
+-- Theorem 7X(b)
+theorem no_2_cyle {a b : Set} : ¬ (a ∈ b ∧ b ∈ a) :=
+begin
+  rintro ⟨ab, ba⟩,
+  have abne : ({a, b} : Set) ≠ ∅, apply ne_empty_of_inhabited, use a, rw [mem_insert], left, refl,
+  obtain ⟨m, mab, miab⟩ := regularity' abne,
+  rw [mem_insert, mem_singleton] at mab, cases mab with ma mb,
+    subst ma, apply mem_empty b, rw [←miab, mem_inter, mem_insert, mem_singleton],
+    exact ⟨ba, or.inr rfl⟩,
+  subst mb, apply mem_empty a, rw [←miab, mem_inter, mem_insert],
+  exact ⟨ab, or.inl rfl⟩,
+end
+
+-- Theorem 7X(c)
+theorem no_ω_cycle : ¬ ∃ f : Set, f.is_function ∧ f.dom = ω ∧ ∀ {n : Set}, n ∈ ω → f.fun_value n.succ ∈ f.fun_value n :=
+begin
+  rintro ⟨f, ffun, fdom, fspec⟩,
+  have ranne : f.ran ≠ ∅, apply ne_empty_of_inhabited, use f.fun_value ∅,
+    apply fun_value_def'' ffun, rw fdom, exact zero_nat,
+  obtain ⟨m, mf, mif⟩ := regularity' ranne,
+  rw mem_ran_iff ffun at mf, rcases mf with ⟨n, nω, mn⟩, subst mn,
+  apply mem_empty (f.fun_value n.succ), rw [←mif, mem_inter, mem_ran_iff ffun],
+  rw fdom at nω, refine ⟨fspec nω, _, _, rfl⟩,
+  rw fdom, exact nat_induct.succ_closed nω,
+end
+
+lemma rank_le_of_subset {x : Set} (xgr : x.grounded) {y : Set} (ygr : y.grounded) (xy : x ⊆ y) : x.rank ≤ y.rank :=
+rank_least_of_grounded xgr (rank_ord_of_grounded ygr) (subset_trans xy (rank_sub_of_grounded ygr))
+
+-- exercise 30(b)
+theorem ch7_p30b {a : Set} : a.powerset.rank = a.rank.succ :=
+begin
+  rw rank_eq_of_all_mem_grounded (λ x h, all_grounded),
+  apply ext, simp only [mem_Union, exists_prop, mem_repl_img, mem_powerset], intro z, split,
+    rintro ⟨w, ⟨x, xa, wx⟩, zw⟩, subst wx, rw mem_succ_iff_le,
+    have zord : z.is_ordinal := ord_of_mem_ord (succ_ord_of_ord (rank_ord_of_grounded all_grounded)) zw,
+    rw ←rank_ord_eq_self zord at *, rw mem_succ_iff_le at zw,
+    apply ord_le_trans (rank_ord_of_grounded all_grounded) zw,
+    exact rank_le_of_subset all_grounded all_grounded xa,
+  intro za, exact ⟨_, ⟨_, subset_self, rfl⟩, za⟩,
+end
+
+-- exercise 30(c)
+theorem ch7_p30c {a : Set} : a.Union.rank ≤ a.rank :=
+begin
+  apply rank_least_of_grounded all_grounded (rank_ord_of_grounded all_grounded),
+  simp only [subset_def, mem_Union, exists_prop], rintro z ⟨x, xa, zx⟩,
+  suffices xa₂ : x.rank.Veb ⊆ a.rank.Veb,
+    apply xa₂, apply rank_sub_of_grounded all_grounded, exact zx,
+  apply Veb_sub_of_mem (rank_ord_of_grounded all_grounded),
+  exact rank_mem_of_mem_grounded all_grounded xa,
+end
+
+-- exercise 33
+theorem ch7_p33 {D : Set} (Dt : D.transitive_set) {B : Set} (BD : ∀ {a : Set}, a ∈ D → a ⊆ B → a ∈ B) : D ⊆ B :=
+begin
+  suffices h : ∀ {α : Set}, α.is_ordinal → D ∩ α.Veb ⊆ B,
+    obtain ⟨α, αord, Dα⟩ := @all_grounded D,
+    rw ←inter_eq_of_sub Dα, exact h αord,
+  apply @trans_ind_schema (λ α, D ∩ α.Veb ⊆ B), intros α αord ind x xDα,
+  rw [mem_inter, mem_Veb αord] at xDα, rcases xDα with ⟨xD, β, βα, xβ⟩,
+  rw transitive_set_iff' at Dt, apply BD xD,
+  exact subset_trans (sub_inter_of_sub (Dt xD) xβ) (ind βα),
+end
+
+-- exercise 35
+theorem succ_inj' {a b : Set} (ab : a.succ = b.succ) : a = b :=
+begin
+  have amb : a ∈ b.succ, rw ←ab, exact self_mem_succ,
+  have bma : b ∈ a.succ, rw ab, exact self_mem_succ,
+  rw [succ, mem_union, mem_singleton] at amb bma,
+  cases bma,
+    symmetry, exact bma,
+  cases amb,
+    exact amb,
+  exfalso, exact no_2_cyle ⟨bma, amb⟩,
+end
+
+lemma eq_iff_le_and_le {a b : Set} : a = b ↔ a ≤ b ∧ b ≤ a :=
+begin
+  split,
+    intro ab, subst ab, exact ⟨or.inr rfl, or.inr rfl⟩,
+  rintro ⟨ab|ab, ba|ba⟩,
+        exfalso, exact no_2_cyle ⟨ab, ba⟩,
+      exact ba.symm,
+    exact ab,
+  exact ab,
+end
+
+-- exercise 38
+theorem limit_ord_eq_Union {γ : Set} (γord : γ.limit_ord) : γ = γ.Union :=
+begin
+  rw eq_iff_subset_and_subset, split,
+    intros α αγ, rw mem_Union,
+    have αγ' : α.succ ∈ γ, apply classical.by_contradiction, intro αγ', apply γord.ns,
+      use α, rw eq_iff_le_and_le,
+      rw ord_not_lt_iff_le (succ_ord_of_ord (ord_of_mem_ord γord.ord αγ)) γord.ord at αγ',
+      exact ⟨αγ', succ_least_upper_bound γord.ord αγ⟩,
+    exact ⟨_, αγ', self_mem_succ⟩,
+  exact (ordinal_trans γord.ord),
+end
+
+end Set
